Mostly complete Fiat4Monitors example.

src/Fiat4Monitors/RADL_Definitions.v
@@ -2,13 +2,15 @@ Require Import
         Coq.Strings.String
         Coq.Bool.Bool
         Coq.Lists.List
+        Coq.Arith.Arith
         Coq.Program.Program
         Fiat.ADT
+        Fiat.ADT.ComputationalADT
         Fiat.ADTNotation
         Fiat.ADTRefinement
         Fiat.ADTRefinement.BuildADTRefinements.
 
-Section RADL_Definitions.
+Section Messages.
 
   Global Open Scope ADT_scope.
   Global Open Scope string_scope.
@@ -22,23 +24,17 @@ Section RADL_Definitions.
   Variable Topics : list RADL_Topic. (* List of Topics in the Network. *)
   Definition TopicID  := @BoundedString (map Topic_Name Topics).
 
-  Record RADL_Node :=
-    { (* Subscription + Publication info for this node *)
-      RADL_Subscriptions : list TopicID;
-      RADL_Publications : list TopicID
-    }.
-
-  Definition RADL_Init := "Init".
-  Definition RADL_Step := "Step".
+  Definition TopicNames
+             (topic : TopicID) : string :=
+    Topic_Name (nth_Bounded Topic_Name Topics topic).
 
   Definition TopicTypes
              (topic : TopicID) : Type :=
     Topic_Type (nth_Bounded Topic_Name Topics topic).
 
-  Definition Message topics :=
-    ilist TopicTypes topics.
+  Definition Message topics := ilist TopicTypes topics.
 
-  Fixpoint SubTopic
+  Fixpoint GetTopic
            (topics : list TopicID)
            {struct topics}
   : Message topics ->
@@ -49,58 +45,320 @@ Section RADL_Definitions.
                   Message topics ->
                   forall (subtopic : BoundedIndex topics),
                     TopicTypes (bindex subtopic) with
-              | nil => fun msg subtopic => BoundedIndex_nil _ subtopic
+              | [ ] => fun msg subtopic => BoundedIndex_nil _ subtopic
               | topic :: topics' =>  fun msg subtopic => _
             end).
     destruct subtopic as [idx [[ | n] nth_n]].
     simpl in *; injection nth_n; intros; subst.
     exact (ith_Bounded id msg {| bindex := _;
                                 indexb := Build_IndexBound (idx :: (map id topics')) 0 nth_n|}).
-    exact (SubTopic topics' (ilist_tl msg) {| bindex := idx;
+    exact (GetTopic topics' (ilist_tl msg) {| bindex := idx;
                        indexb := {| ibound := n;
                                     boundi := nth_n |} |} ).
   Defined.
 
-  Fixpoint SubMessage
+  Fixpoint SetTopic
+           (topics : list TopicID)
+           {struct topics}
+  : Message topics ->
+    forall (subtopic : BoundedIndex topics),
+      TopicTypes (bindex subtopic) ->
+      Message topics.
+  Proof.
+    refine (match topics return
+                  Message topics ->
+                  forall (subtopic : BoundedIndex topics),
+                    TopicTypes (bindex subtopic) -> Message topics with
+              | [ ] => fun msg subtopic val => inil _
+              | topic :: topics' =>  fun msg subtopic val => _
+            end).
+    destruct subtopic as [idx [[ | n] nth_n]].
+    - simpl in *; injection nth_n; intros; subst;
+      exact (icons _ val (ilist_tl msg)).
+    - exact (icons _ (ilist_hd msg) (SetTopic topics' (ilist_tl msg)
+                                              {| bindex := idx;
+                                                 indexb := {| ibound := n;
+                                                              boundi := nth_n |} |}
+                                              val)).
+  Defined.
+
+  Section RADL_MessageADT.
+
+    Open Scope methSig.
+    Open Scope consSig.
+    Open Scope cMethDef.
+    Open Scope cConsDef.
+
+    (* Message Initialization *)
+    Definition Message_Init := "Init".
+
+    Fixpoint InitMessageDom (topics : list TopicID) :=
+      match topics return Type with
+        | [ ] => unit
+        | topic :: topics' => prod (TopicTypes topic) (InitMessageDom topics')
+      end.
+
+    Definition InitMessageSig (topics : list TopicID) : consSig :=
+      Constructor Message_Init : InitMessageDom topics -> rep.
+
+    Fixpoint InitMessage (topics : list TopicID)
+    : InitMessageDom topics -> Message topics :=
+      match topics return
+            InitMessageDom topics -> Message topics with
+        | [ ] =>
+          fun inits => inil _
+        | topic :: topics' =>
+          fun inits => icons _ (fst inits) (InitMessage topics' (snd inits))
+      end.
+
+    Definition InitMessageDef (topics : list TopicID) :=
+      Def Constructor Message_Init (inits : InitMessageDom topics) : rep :=
+      InitMessage topics inits.
+
+    (* Getters and Setters for Messages *)
+    Variable topics : list TopicID.
+
+    Definition GetMessageSig (topic : BoundedIndex topics) :=
+      Method ("Get" ++ TopicNames (bindex topic)) : rep x unit -> rep x TopicTypes (bindex topic).
+
+    Definition SetMessageSig (topic : BoundedIndex topics) :=
+      Method ("Set" ++ TopicNames (bindex topic)) : rep x TopicTypes (bindex topic) -> rep x unit.
+
+    Fixpoint MessageSigs (subtopics : list (BoundedIndex topics)) : list methSig :=
+      match subtopics with
+        | [ ] => [ ]
+        | topic :: topics' =>
+          GetMessageSig topic :: SetMessageSig topic :: MessageSigs topics'
+      end.
+
+    Definition GetMessageDef (topic : BoundedIndex topics) :
+      cMethDef (Rep := Message topics) (GetMessageSig topic) :=
+      Def Method _ (msg : rep, _ : _) : TopicTypes (bindex topic) :=
+      (msg, GetTopic msg topic).
+
+    Definition SetMessageDef (topic : BoundedIndex topics) :
+      cMethDef (Rep := Message topics) (SetMessageSig topic) :=
+      Def Method _ (msg : rep, val : TopicTypes (bindex topic)) : unit :=
+      (SetTopic msg _ val, tt).
+
+    Fixpoint MessageDefs'
+             (subtopics : list (BoundedIndex topics))
+    : ilist (cMethDef (Rep := Message topics)) (MessageSigs subtopics) :=
+      match subtopics return
+            ilist (cMethDef (Rep := Message topics)) (MessageSigs subtopics) with
+        | [ ] => inil _
+        | topic :: subtopics' =>
+          icons _ (GetMessageDef topic) (icons _ (SetMessageDef topic) (MessageDefs' subtopics'))
+      end.
+
+    Definition LiftTopics : list (BoundedIndex topics) :=
+      (fix LiftTopics (topics : list TopicID) : list (BoundedIndex topics) :=
+         match topics with
+           | [ ] => [ ]
+           | topic :: topics' =>
+             {| bindex := _; indexb := IndexBound_head _ _ |}
+               :: (map (fun idx : BoundedIndex topics' =>
+                          {| bindex := bindex idx;
+                             indexb := @IndexBound_tail _ _ topic _ (indexb idx) |})
+                       (LiftTopics topics'))
+         end) topics.
+
+    Definition MessageDefs := MessageDefs' LiftTopics.
+
+    (* Message ADT Definitions *)
+    Definition MessageADTSig : ADTSig :=
+      BuildADTSig [InitMessageSig topics] (MessageSigs LiftTopics).
+
+    Definition MessageADT : cADT MessageADTSig :=
+      BuildcADT (icons _ (InitMessageDef topics) (inil _)) MessageDefs.
+
+    (* Support for building messages. *)
+
+    Definition ConstructMessage (msg : cADT (MessageADTSig)) subtopics :=
+      CallConstructor msg Message_Init subtopics.
+
+    (* Support for calling message getters. *)
+    Definition BuildGetMethodID'
+               (subtopics : list (BoundedIndex topics))
+               (idx : BoundedIndex (map (fun id => bindex id) subtopics))
+    : @BoundedString (map methID (MessageSigs subtopics)).
+      refine {| bindex := ("Get" ++ (bindex (bindex idx)))%string;
+                indexb := {| ibound := 2 * ibound idx;
+                             boundi := _ |}
+             |}.
+      destruct idx as [idx [n nth_n]].
+      revert idx n nth_n; induction subtopics; intros.
+      destruct n; simpl in *; discriminate.
+      destruct n; simpl in *.
+      - unfold value; repeat f_equal.
+        destruct a as [b [m nth_m]]; simpl in *; subst.
+        unfold TopicNames; injections.
+        destruct idx as [topic [p nth_p]]; simpl in *.
+        pose proof (nth_error_map _ _ _ nth_p).
+        cut (exists topic'', nth_error Topics p = Some topic'' /\ Topic_Name topic'' = topic ).
+        intros.
+        eapply nth_Bounded_ind; intros.
+        subst filtered_var program_branch_0 program_branch_1; simpl.
+        destruct_ex; intuition.
+        rewrite H1; eauto.
+        revert H; clear.
+        destruct (nth_error Topics p); intros;
+        first [discriminate | injections; eauto].
+      - rewrite plus_comm; simpl; rewrite plus_comm.
+        eauto.
+    Defined.
+
+    Definition BuildGetMethodID
+               (idx : BoundedIndex (map (fun id => bindex id) LiftTopics))
+    : @BoundedString (map methID (MessageSigs LiftTopics))
+      := BuildGetMethodID' _ idx.
+
+    Definition CallMessageGetMethod
+               (r : Message topics)
+               idx
+      := cMethods MessageADT (BuildGetMethodID idx) r.
+
+    (* Support for calling message setters. *)
+    Definition BuildSetMethodID'
+             (subtopics : list (BoundedIndex topics))
+             (idx : BoundedIndex (map (fun id => bindex id) subtopics))
+  : @BoundedString (map methID (MessageSigs subtopics)).
+    Proof.
+      refine {| bindex := ("Set" ++ (bindex (bindex idx)))%string;
+                indexb := {| ibound := 2 * ibound idx + 1;
+                             boundi := _ |}
+             |}.
+      destruct idx as [idx [n nth_n]].
+      revert idx n nth_n; induction subtopics; intros.
+      destruct n; simpl in *; discriminate.
+      destruct n; simpl in *.
+      - unfold value; repeat f_equal.
+        destruct a as [b [m nth_m]]; simpl in *; subst.
+        unfold TopicNames; injections.
+        destruct idx as [topic [p nth_p]]; simpl in *.
+        pose proof (nth_error_map _ _ _ nth_p).
+        cut (exists topic'', nth_error Topics p = Some topic'' /\ Topic_Name topic'' = topic ).
+        intros.
+        eapply nth_Bounded_ind; intros.
+        subst filtered_var program_branch_0 program_branch_1; simpl.
+        destruct_ex; intuition.
+        rewrite H1; eauto.
+        revert H; clear.
+        destruct (nth_error Topics p); intros;
+        first [discriminate | injections; eauto].
+      - rewrite plus_comm; simpl.
+        rewrite <- (IHsubtopics idx n nth_n); f_equal.
+        omega.
+    Defined.
+
+    Definition BuildSetMethodID
+               (idx : BoundedIndex (map (fun id => bindex id) LiftTopics))
+    : @BoundedString (map methID (MessageSigs LiftTopics))
+      := BuildSetMethodID' _ idx.
+
+    Definition CallMessageSetMethod (r : Message topics) idx :=
+      cMethods MessageADT (BuildSetMethodID idx) r.
+
+  End RADL_MessageADT.
+
+  (* Support for calling message constructors. *)
+
+  Fixpoint SubMessageDom
+           (topics : list TopicID)
+           (subtopics : list (BoundedIndex topics))
+           (msg : Message topics)
+    : InitMessageDom (map (bindex (Bound := topics)) subtopics) :=
+      match subtopics return InitMessageDom (map (bindex (Bound := topics)) subtopics) with
+        | [ ] => ()
+        | subtopic :: subtopics' =>
+          (GetTopic msg subtopic, SubMessageDom subtopics' msg)
+      end.
+
+  Definition SubMessage
              (topics : list TopicID)
-             (subtopics : list (BoundedIndex  topics))
+             (subtopics : list (BoundedIndex topics))
              (msg : Message topics)
-  : Message (map (bindex (Bound := topics)) subtopics) :=
-    match subtopics return Message (map (bindex (Bound := topics)) subtopics) with
-      | nil => inil _
-      | subtopic :: subtopics' =>
-        icons _ (SubTopic msg subtopic )
-              (SubMessage subtopics' msg)
-    end.
+  : cRep (MessageADT (map (bindex (Bound := topics)) subtopics)) :=
+    cConstructors (MessageADT (map (bindex (Bound := topics)) subtopics))
+                  ``Message_Init
+                  (SubMessageDom subtopics msg).
+
+  Section RADL_ADT.
+
+  Definition RADL_Init := "Init".
+  Definition RADL_Step := "Step".
+
+  Record RADL_Node :=
+    { (* Subscription + Publication info for this node *)
+      RADL_Subscriptions : list TopicID;
+      RADL_Publications : list TopicID
+    }.
+
+  Definition radl_in_t (Node : RADL_Node) := MessageADT (RADL_Subscriptions Node).
+  Definition radl_out_t (Node : RADL_Node) := MessageADT (RADL_Publications Node).
 
   Definition RADL_ADTSig  (Node : RADL_Node)
   : ADTSig :=                         (* A RADL Node is modeled as an ADT with a  *)
     ADTsignature {                    (* single constructor and a step function. *)
         Constructor RADL_Init      : unit -> rep,
-        Method      RADL_Step      : rep x Message (RADL_Subscriptions Node)
-                                     -> rep x Message (RADL_Publications Node)
+        Method      RADL_Step      : rep x cRep (radl_in_t Node)
+                                     -> rep x cRep (radl_out_t Node)
       }.
 
-  Definition RADL_ADTSpec (Node : RADL_Node)
+    Definition RADL_ADTSpec (Node : RADL_Node)
   : ADT (RADL_ADTSig Node) :=
     ADTRep unit (* Since RADL Nodes are untrusted, we'll treat their state as completely unknown *)
            { Def Constructor RADL_Init (_ : unit) : rep := ret tt,
-             Def Method RADL_Step (r : rep, in_t : Message (RADL_Subscriptions Node)) : _ :=
+             Def Method RADL_Step (r : rep, in_t : cRep (radl_in_t Node)) : _ :=
                (* Again, since the RADL Node is untrusted code, we'll assume that it can publish
                   whatever the heck it wants. *)
-               results <- {out_t : Message (RADL_Publications Node) | True };
+               results <- {out_t : cRep (radl_out_t Node) | True };
              ret (tt, results) }.
 
+  Record RADLM_Node :=
+    { (* The model of the monitor's internal state *)
+      RADLM_Rep : Type;
+      (* The monitored node*)
+      RADLM_MonitoredNode : RADL_Node;
+      (* Additional Subscription + Publication info *)
+      RADLM_Subscriptions : list TopicID;
+      RADLM_Publications : list TopicID
+    }.
+
+  Definition radlm_in_t (Node : RADLM_Node) :=
+    MessageADT (RADL_Subscriptions (RADLM_MonitoredNode Node)).
+  Definition radlm_out_t (Node : RADLM_Node) :=
+    MessageADT (RADL_Publications (RADLM_MonitoredNode Node)).
+  Definition radlm_monitor_in_t (Node : RADLM_Node) :=
+    MessageADT (RADLM_Subscriptions Node).
+  Definition radlm_monitor_out_t (Node : RADLM_Node) :=
+    MessageADT (RADLM_Publications Node).
+
   Definition RADLM_ADTSig
-             (MonitorNode : RADL_Node)
+             (MonitorNode : RADLM_Node)
              (InitDom : Type)
   : ADTSig :=
     ADTsignature {
         Constructor RADL_Init      : InitDom -> rep,
-        Method      RADL_Step      : rep x unit * Message (RADL_Subscriptions MonitorNode)
-                                     -> rep x unit * Message (RADL_Publications MonitorNode)
+        Method      RADL_Step      : rep x unit * cRep (radlm_in_t MonitorNode) * cRep (radlm_monitor_in_t MonitorNode)
+                                     -> rep x unit
+                                        * cRep (radlm_out_t MonitorNode)
+                                        * cRep (radlm_monitor_out_t MonitorNode)
       }.
 
-End RADL_Definitions.
+  End RADL_ADT.
+End Messages.
 
-Notation GetTopic il idx := (SubTopic il ``(``idx)).
+Notation "r '~~>' idx " := (CallMessageGetMethod r {|bindex := ``idx; indexb := _ |} tt)
+                              (idx at level 0, at level 70).
+
+(* Notation to automatically inject subtopics into TopicIDs in SubMessage*)
+Delimit Scope SubMessage_scope with SubMessage.
+
+Notation "[ msg1 ; .. ; msgn ]" :=
+  (cons (``(``(msg1%string))) .. (cons (``(``(msgn%string))) nil) ..) : SubMessage_scope.
+
+Global Arguments SubMessage {Topics topics} subtopics%SubMessage msg.
+
+Hint Extern 0 (IndexBound _ (map _ _)) =>
+progress simpl; eauto with typeclass_instances : typeclass_instances.
