src/Fiat4Monitors/TurretMonitor.v
@@ -1,164 +1,83 @@
-Set Implicit Arguments.
-
-Require Import Coq.Lists.List Coq.Program.Program.
+Require Import Coq.Lists.List Coq.Program.Program Coq.Arith.Arith.
+Require Import Fiat.Fiat4Monitors.RADL_Definitions
+        Fiat.Fiat4Monitors.TurretMonitorSpec
+        Fiat.Fiat4Monitors.MonitorADTs
+        Fiat.Fiat4Monitors.MonitorRepInv
+        Fiat.ADT
+        Fiat.ADT.ComputationalADT
+        Fiat.ADTNotation
+        Fiat.ADTRefinement
+        Fiat.ADTRefinement.BuildADTRefinements.
 Require Import Bedrock.Platform.Facade.DFacade.
 Require Import Bedrock.Platform.Facade.Notations.
 Require Import Bedrock.Platform.Cito.ADT.
 Require Import Bedrock.Platform.Cito.RepInv.
 
-(* From a RADL description, SRI generates structs aggregating
-   incoming and outgoing messages for each node. These records are
-   used to model those structs as ADTs. *)
+Definition GetTiltXSpec :=
+  Message_Monitor_In_SetSpec (PaintballMonitorSpec (fun _ => true)
+                                                   (fun _ => true))
+                                                   ````"TiltX" id id.
+Definition GetTiltYSpec :=
+  Message_Monitor_In_SetSpec (PaintballMonitorSpec (fun _ => true)
+                                                   (fun _ => true))
+                             ````"TiltY" id id.
+Definition Monitored_Node_StepSpec :=
+  RADL_Monitored_Node_StepSpec (PaintballMonitorSpec (fun _ => true)
+                                                     (fun _ => true)).
+Definition Monitor_Init_Spec := 
+  MonitorNode_InitSpec (PaintballMonitorSpec (fun _ => true)
+                                             (fun _ => true)).
+Definition Monitor_Step_Spec := 
+  MonitorNode_StepSpec (PaintballMonitorSpec (fun _ => true)
+                                             (fun _ => true)).
 
-(* Incoming messages to paintball node. (Subscribes to the trigger.)  *)
-Record radl_in_t :=
-  { trigger : Memory.B (* uint8 *) }.
-
-(* Not sure what these flags represent. *)
-Record radl_in_flag_t :=
-  { radl_flags : Memory.B (* uint8 *) }.
-
-(* Outgoing messages to paintball node. (Doesn't publish anything.)  *)
-Record radl_out_t := { }.
-Record radl_out_flag_t := { }.
-
-(* Incoming messages to paintball monitor node. (Subscribes to the turret's
-   tilt sensor.)  *)
-Record monitor_in_t :=
-  { tilt : Memory.W  * Memory.W (* float64 *) }.
-
-Record monitor_out_t :=
-  {  }.
-
-(* Each of these structs is represented in Facade as a distinct ADT. *)
-Inductive PaintballADTValues :=
-| RADL_In : radl_in_t -> PaintballADTValues
-| RADL_In_Flags : radl_in_flag_t -> PaintballADTValues
-| RADL_Out : radl_out_t -> PaintballADTValues
-| RADL_Out_Flags : radl_out_flag_t -> PaintballADTValues
-| Monitor_In : monitor_in_t -> PaintballADTValues
-| Monitor_In_Flags : monitor_in_flag_t -> PaintballADTValues.
-
-Module Adt <: ADT.
-  Definition ADTValue := PaintballADTValues.
-End Adt.
-
-Ltac crush_types :=
-  unfold type_conforming, same_types, same_type; intros;
-  repeat match goal with
-           | [ H: exists t, _ |- _ ] => destruct H
-         end; subst;
-  intuition.
-
-(* Specs for getters for our ADTValues. *)
-Definition monitor_in_tilt1Spec : AxiomaticSpec PaintballADTValues.
-  refine {|
-      PreCond args := exists w w', args = [ADT (Monitor_In {| tilt := (w, w') |})];
-      PostCond args ret :=
-        exists w w', args = [(ADT (Monitor_In {| tilt := (w, w') |}),
-                              Some (Monitor_In {| tilt := (w, w') |})) ] /\
-                     ret = SCA _ w
-    |}; crush_types.
-Defined.
-
-Definition monitor_in_tilt2Spec : AxiomaticSpec PaintballADTValues.
-  refine {|
-    PreCond args := exists w w', args = [ADT (Monitor_In {| tilt := (w, w') |})];
-    PostCond args ret :=
-      exists w w', args = [(ADT (Monitor_In {| tilt := (w, w') |}),
-                            Some (Monitor_In {| tilt := (w, w') |})) ] /\
-                   ret = SCA _ w'
-  |}; crush_types.
-Defined.
-
-Definition radl_in_triggerSpec : AxiomaticSpec PaintballADTValues.
-  refine {|
-      PreCond args :=
-        exists w w',
-          args = [ADT (RADL_In {| trigger := w |});
-                   ADT (RADL_In_Flags {| radl_flags := w' |});
-                   ADT (RADL_Out Build_radl_out_t);
-                   ADT (RADL_Out_Flags Build_radl_out_flag_t )];
-      PostCond args ret :=
-        exists w w', args = [(ADT (RADL_In {| trigger := w |}),
-                              Some (RADL_In {| trigger := w |}));
-                              (ADT (RADL_In_Flags {| radl_flags := w' |}),
-                               Some (RADL_In_Flags {| radl_flags := w |}));
-                              (ADT (RADL_Out Build_radl_out_t),
-                               Some (RADL_Out Build_radl_out_t));
-                              (ADT (RADL_Out_Flags Build_radl_out_flag_t ),
-                               Some (RADL_Out_Flags Build_radl_out_flag_t ))
-
-                            ] /\
-                     ret = SCA _ w
-    |}; crush_types.
-Defined.
-
-Definition paintball_monitor_step_spec : AxiomaticSpec PaintballADTValues.
-  refine {|
-      PreCond args :=
-        exists w w' tilt_x tilt_y w'',
-          args = [ ADT (RADL_In {| trigger := w |});
-                   ADT (RADL_In_Flags {| radl_flags := w' |});
-                   ADT (RADL_Out Build_radl_out_t);
-                   ADT (RADL_Out_Flags Build_radl_out_flag_t );
-                   ADT (Monitor_In {| tilt := (tilt_x, tilt_y) |});
-                   ADT (Monitor_In_Flags {| monitor_flags := w'' |}) ];
-      PostCond args ret :=
-        exists w w', args = [(ADT (RADL_In {| trigger := w |}),
-                              Some (RADL_In {| trigger := w |}));
-                              (ADT (RADL_In_Flags {| radl_flags := w' |}),
-                               Some (RADL_In_Flags {| radl_flags := w |}));
-                              (ADT (RADL_Out Build_radl_out_t),
-                               Some (RADL_Out Build_radl_out_t));
-                              (ADT (RADL_Out_Flags Build_radl_out_flag_t ),
-                               Some (RADL_Out_Flags Build_radl_out_flag_t ))
-
-                                     ] /\
-                                 ret = SCA _ w
-    |}. crush_types.
-Defined.
-
-Import Bedrock.Platform.Facade.Notations.OpenScopes.
+  Import Bedrock.Platform.Facade.Notations.OpenScopes.
 
 Definition paintball_monitor :=
   module
   import {
-      "ADT"!"RADL_In_Trigger" ==> radl_in_triggerSpec;
-      "ADT"!"Monitor_In_Tilt1" ==> monitor_in_tilt1Spec;
-      "ADT"!"Monitor_In_Tilt2" ==> monitor_in_tilt2Spec
+      "ADT"!"GetTiltX" ====> GetTiltXSpec;
+      "ADT"!"GetTiltY" ====> GetTiltYSpec;
+      "ADT"!"Node_Step" ====> Monitored_Node_StepSpec
     }
     define {
-      def "step" = func("in", "in_flags", "out", "out_flags", "monitor_in", "monitor_out") {
-        "tilt_x" <-- call_ "ADT"!"Monitor_In_Tilt1"("monitor_in");
-        "tilt_y" <-- call_ "ADT"!"Monitor_In_Tilt2"("monitor_in");
+      def "init" = func() {"ret" <-- call_ "ADT"!"BuildUnit" () };
+      
+      def "step" = func("node", "in", "out", "monitor_in", "monitor_out") {
+        "tilt_x" <-- call_ "ADT"!"GetTiltX"("monitor_in");
+        "tilt_y" <-- call_ "ADT"!"GetTiltY"("monitor_in");
         if_ ("tilt_x" < 10) {
-           if_ ("tilt_y" < 20) {
-                 "ret" <-- call_ "ADT"!"RADL_In_Trigger" ("in", "in_flags", "out", "out_flags")
-           } { "ret" <- 0 } } { "ret" <- 0 } }
-    }.
+              if_ ("tilt_y" < 20) {
+                    "ret" <-- call_ "ADT"!"Node_Step" ("node", "in", "out")
+                  }
+                  { "ret" <-- call_ "ADT"!"Node_Step" ("node", "in", "out") } }
+            { "ret" <-- call_ "ADT"!"Node_Step" ("node", "in", "out") }
+            } }.
+Require Import Bedrock.Platform.Facade.CompileUnit2.
 
-  Require Import Bedrock.Platform.Facade.CompileDFModule.
+Definition paintball_monitor_exports :=
+  StringMap.StringMap.add "init"  Monitor_Init_Spec
+                          (StringMap.StringMap.add "step"  Monitor_Step_Spec (StringMap.StringMap.empty _)).
 
-  Definition gmodule
-    := compile_to_gmodule (paintball_monitor eq_refl) "paintball_monitor" eq_refl.
+Definition paintball_monitor_module
+: CompileUnit paintball_monitor_exports.
+  eapply (@Build_CompileUnit _ paintball_monitor_exports (paintball_monitor eq_refl) "paintball_monitor_ax" "paintball_monitor"); eauto.
+Defined.
 
-  (* test executability *)
-  Require Import Bedrock.Platform.Cito.GoodModuleDec.
-  Require Import Bedrock.Platform.Cito.IsGoodModule.
+Require Import Bedrock.Platform.Facade.CompileDFModule.
+Require Import Bedrock.Platform.Facade.DFacadeToBedrock2.
 
-  Goal is_good_module gmodule = true. Proof. exact eq_refl. Qed.
+Module Import M := DFacadeToBedrock2.Make MonitorADTs.Adt MonitorRepInv.Ri .
 
-  Require Import Bedrock.Platform.Facade.CompileUnit2.
+Definition output := compile paintball_monitor_module.
+Definition m1 := CompileOut2.bedrock_module output.
+Definition m1_ok := CompileOut2.bedrock_module_ok output.
+Definition m2 := CompileOut2.bedrock_module_impl output.
+Definition m2_ok := CompileOut2.bedrock_module_impl_ok output.
+Definition all1 := link m1 m2.
 
-  Definition paintball_monitor_exports :
-    StringMap.StringMap.t (AxiomaticSpec PaintballADTValues).
+(* I don't have enough memory to test this linking :( *)
+Lemma all1_ok : moduleOk all1.
+    link m1_ok m2_ok.
+Qed.
 
-    refine (StringMap.StringMap.add "step" _ (StringMap.StringMap.empty _)).
-    Print AxiomaticSpec.
-
-
-  Definition paintball_monitor_compileUnit :
-    CompileUnit PaintballADTValues.
-
-End ADTValue.
