src/Fiat4Monitors/TurretMonitorSpec.v
@@ -1,8 +1,20 @@
-Section Paintball.
+Require Import
+        Coq.Strings.String
+        Coq.Bool.Bool
+        Coq.Lists.List
+        Coq.Program.Program
+        Fiat.ADT
+        Fiat.ADT.ComputationalADT
+        Fiat.ADTNotation
+        Fiat.ADTRefinement
+        Fiat.ADTRefinement.BuildADTRefinements
+        Fiat.Fiat4Monitors.RADL_Definitions.
+
+Section Example.
 
   Require Bedrock.Platform.Facade.DFacade.
 
-  Definition PaintballControlMode :=
+  Definition PaintballControlMode : Set :=
     @BoundedString ["IDLE"; "SINGLE_SHOT"; "TRIPLE_SHOT"; "BURST"].
 
   (* This is the list of topics available in the system.*)
@@ -14,28 +26,28 @@ Section Paintball.
 
   (* Each RADL Node has a list of subscriptions and publications drawn
      from the list of available topics. *)
-  Definition BarrelNode : RADL_Node PaintballTopics :=
+  Definition PaintballNode : RADL_Node PaintballTopics :=
     {| RADL_Subscriptions := [ ``"Trigger"];
        RADL_Publications  := [ ``"Fired"] |}.
   Definition TurretNode : RADL_Node PaintballTopics :=
     {| RADL_Subscriptions := [ ];
        RADL_Publications  := [``"TiltX"; ``"TiltY"] |}.
-  Definition TriggerNode : RADL_Node PaintballTopics :=
+  Definition JoystickNode : RADL_Node PaintballTopics :=
     {| RADL_Subscriptions := [ ];
        RADL_Publications  := [ ``"Trigger"] |}.
 
   (* Each RADL Node has a default implementation that nondeterministically
      selects a publication value (since the underlying RADL Nodes are
      untrusted code). *)
-  Definition BarrelSpec : Core.ADT (RADL_ADTSig BarrelNode) :=
-    RADL_ADTSpec BarrelNode.
+  Definition PaintballSpec : Core.ADT (RADL_ADTSig PaintballNode) :=
+    RADL_ADTSpec PaintballNode.
   Definition TurretSpec : Core.ADT (RADL_ADTSig TurretNode) :=
     RADL_ADTSpec TurretNode.
-  Definition TriggerSpec : Core.ADT (RADL_ADTSig TriggerNode) :=
-    RADL_ADTSpec TriggerNode.
+  Definition JoystickSpec : Core.ADT (RADL_ADTSig JoystickNode) :=
+    RADL_ADTSpec JoystickNode.
 
   Definition PaintballTopicIDs :=
-    RADL_Publications TurretNode ++ RADL_Publications TriggerNode ++ RADL_Publications BarrelNode.
+    RADL_Publications TurretNode ++ RADL_Publications JoystickNode ++ RADL_Publications PaintballNode.
 
   (* Guard functions which check if the turret is pointed in a safe direction. *)
   Variables TiltXSafe TiltYSafe : Memory.W -> bool.
@@ -43,188 +55,149 @@ Section Paintball.
   (* The complete specification is an ADT that has a single constructor that initializes the
      RADL Nodes and a single step function that checks a global condition on each topic,
      calling the original step functions if it holds and does some error handling otherwise. *)
-  Definition PaintballSpec :=
-    ADTRep (Rep BarrelSpec * Rep TurretSpec * Rep TriggerSpec)
-                   { Def Constructor RADL_Init (_ : unit) : rep :=
-                       barrel <- callCons BarrelSpec RADL_Init tt;
-                       turret <- callCons TurretSpec RADL_Init tt;
-                       trigger <- callCons TriggerSpec RADL_Init tt;
-                       ret (barrel, turret, trigger),
 
-                     Def Method RADL_Step (r : rep, in_t : Message PaintballTopicIDs) :
-                         (* Right now, we have a single, global guard that determines whether
-                            to call the original step functions. *)
-                       Message PaintballTopicIDs :=
-                         if (TiltXSafe (GetTopic in_t "TiltX")
-                                       && TiltYSafe (GetTopic in_t "TiltY")) then
-                           (* Call the original step functions. *)
-                           barrel <- callMeth BarrelSpec RADL_Step (fst (fst r)) (SubMessage [````"Trigger" ] in_t);
-                           turret <- callMeth TurretSpec RADL_Step (snd (fst r)) (SubMessage [] in_t);
-                           trigger <- callMeth TriggerSpec RADL_Step (snd r) (SubMessage [] in_t);
-                           ret ((fst barrel, fst turret, fst trigger),
-                                (ilist_app (snd turret) (ilist_app (snd trigger) (snd barrel))))
-                         else
-                           (* The failure case calls the trigger and turret step functions
+  Open Scope ADTParsing_scope.
+  Definition EveryMessage := Message PaintballTopicIDs.
+
+  Definition ExampleSpec :=
+    ADTRep (Rep PaintballSpec * Rep TurretSpec * Rep JoystickSpec)
+     { Def Constructor RADL_Init (_ : unit) : rep :=
+         barrel <- callCons PaintballSpec RADL_Init tt;
+         turret <- callCons TurretSpec RADL_Init tt;
+         trigger <- callCons JoystickSpec RADL_Init tt;
+         ret (barrel, turret, trigger),
+       Def Method RADL_Step (r' : rep, msg : EveryMessage) : EveryMessage  :=
+           if (TiltXSafe (snd (msg ~~> "TiltX"))
+                         && TiltYSafe (snd (msg ~~> "TiltY"))) then
+             (* Call the original step functions. *)
+             barrel <- callMeth PaintballSpec RADL_Step (fst (fst r')) (SubMessage ["Trigger" ] msg);
+             turret <- callMeth TurretSpec RADL_Step (snd (fst r')) (SubMessage [] msg);
+             trigger <- callMeth JoystickSpec RADL_Step (snd r') (SubMessage [] msg);
+             ret ((fst barrel, fst turret, fst trigger),
+                  (ilist_app (snd turret) (ilist_app (snd trigger) (snd barrel))))
+           else
+             (* The failure case calls the trigger and turret step functions
                               and publishes "IDLE" for the barrel node. *)
-                           trigger <- callMeth TriggerSpec RADL_Step (fst (fst r)) (SubMessage [] in_t);
-                       turret <- callMeth TurretSpec RADL_Step (snd (fst r)) (SubMessage [] in_t);
-                       ret ((tt, fst turret, fst trigger),
-                            (ilist_app (snd turret) (ilist_app (snd trigger)
-                                                               ((icons (B := @TopicTypes PaintballTopics)(``"Fired") ``("IDLE") (inil _))))))}.
+             trigger <- callMeth JoystickSpec RADL_Step (fst (fst r')) (SubMessage [] msg);
+         turret <- callMeth TurretSpec RADL_Step (snd (fst r')) (SubMessage [] msg);
+         ret ((tt, fst turret, fst trigger),
+              (ilist_app (snd turret) (ilist_app (snd trigger)
+                                                 ((icons (B := @TopicTypes PaintballTopics)(``"Fired") ``("IDLE") (inil _))))))}.
 
   (* We now define the publication and subscription information for
      and the specs of the monitor nodes. *)
-  Definition BarrelMonitorNode : RADL_Node PaintballTopics :=
-    {| RADL_Subscriptions := [ ``"Trigger"; ``"TiltX"; ``"TiltY"];
-       RADL_Publications  := [ ``"Fired"] |}.
+  Definition PaintballMonitorNode : RADLM_Node PaintballTopics :=
+    {| RADLM_Rep := unit;
+       RADLM_MonitoredNode := PaintballNode;
+       RADLM_Subscriptions := [ ``"TiltX"; ``"TiltY" ];
+       RADLM_Publications  := [ ] |}.
 
-  Definition TurretMonitorNode : RADL_Node PaintballTopics :=
-    {| RADL_Subscriptions := [ ];
-       RADL_Publications  := [ ``"TiltX"; ``"TiltY"] |}.
+  Definition TurretMonitorNode : RADLM_Node PaintballTopics :=
+    {| RADLM_Rep := unit;
+       RADLM_MonitoredNode := TurretNode;
+       RADLM_Subscriptions := [ ];
+       RADLM_Publications  := [ ] |}.
 
-  Definition TriggerMonitorNode : RADL_Node PaintballTopics :=
-    {| RADL_Subscriptions := [ ];
-       RADL_Publications  := [ ``"Trigger"] |}.
+  Definition JoystickMonitorNode : RADLM_Node PaintballTopics :=
+    {| RADLM_Rep := unit;
+       RADLM_MonitoredNode := JoystickNode;
+       RADLM_Subscriptions := [ ];
+       RADLM_Publications  := [ ] |}.
 
   (* The specs distribute the global monitor to each monitor node.
      In the case of the barrel, the monitor checks the turret position
-     before calling the original step function. *)
-  Definition BarrelMonitorSpec : Fiat.ADT.Core.ADT (RADLM_ADTSig BarrelMonitorNode unit) :=
+     before calling the original step function. Synthesizing the following
+     specs during a derivation is our eventual goal. *)
+
+  Definition PaintballMonitor_Output :=
+    (unit * cRep (radlm_out_t PaintballMonitorNode) * cRep (radlm_monitor_out_t PaintballMonitorNode))%type.
+
+  Definition PaintballMonitorSpec : Fiat.ADT.Core.ADT (RADLM_ADTSig PaintballMonitorNode unit) :=
     ADTRep unit
            { Def Constructor RADL_Init (_ : unit) : rep := ret tt,
-             Def Method RADL_Step (r : rep, in_t : unit * Message (RADL_Subscriptions BarrelMonitorNode)) : _ :=
-               if (TiltXSafe (GetTopic (snd in_t) "TiltX")
-                             && TiltYSafe (GetTopic (snd in_t) "TiltY")) then
-                 barrel <- callMeth BarrelSpec RADL_Step (fst in_t)
-                         (SubMessage [````"Trigger" ] (snd in_t))
-                 ;
-                 ret (tt, barrel)
+             Def Method RADL_Step (r : rep, msg : unit * cRep (radlm_in_t PaintballMonitorNode) * cRep (radlm_monitor_in_t PaintballMonitorNode)) : PaintballMonitor_Output :=
+               if (TiltXSafe (snd (snd msg ~~> "TiltX"))
+                             && TiltYSafe (snd (snd msg ~~> "TiltY"))) then
+                 barrel <- callMeth PaintballSpec RADL_Step (fst (fst msg))
+                        (SubMessage ["Trigger" ] (snd (fst (msg))));
+                 ret (tt, (barrel, inil _))
                else
-                 ret (tt, (tt, (icons (B := @TopicTypes PaintballTopics)(``"Fired") ``("IDLE") (inil _))))
+                 ret (tt, (fst (fst msg), ConstructMessage (radlm_out_t PaintballMonitorNode)
+                                                (``"IDLE", ()), inil _))
            }.
 
   (* The other two monitor nodes don't have to check anything to enforce the guard. *)
-  Definition TurretMonitorSpec : Fiat.ADT.Core.ADT (RADLM_ADTSig TurretNode unit) :=
+  Definition TurretMonitor_Output :=
+    (unit * cRep (radlm_out_t TurretMonitorNode) * cRep (radlm_monitor_out_t TurretMonitorNode))%type.
+
+  Definition TurretMonitorSpec : Fiat.ADT.Core.ADT (RADLM_ADTSig TurretMonitorNode unit) :=
     ADTRep unit
            { Def Constructor RADL_Init (_ : unit) : rep := ret tt,
-             Def Method RADL_Step (r : rep, in_t : unit * Message (RADL_Subscriptions TurretMonitorNode)) : _ :=
-               turret <- callMeth TurretSpec RADL_Step (fst in_t) (snd in_t);
-             ret (tt, turret)
+             Def Method RADL_Step (r : rep, msg : unit * cRep (radlm_in_t TurretMonitorNode) * cRep (radlm_monitor_in_t TurretMonitorNode)) : TurretMonitor_Output :=
+               turret <- callMeth TurretSpec RADL_Step (fst (fst msg)) (snd (fst msg));
+             ret (tt, (turret, inil _ ))
            }.
 
-  Definition TriggerMonitorSpec : Fiat.ADT.Core.ADT (RADLM_ADTSig TriggerNode unit) :=
-    ADTRep unit
+  Definition JoystickMonitor_Output :=
+    (unit * cRep (radlm_out_t JoystickMonitorNode) * cRep (radlm_monitor_out_t JoystickMonitorNode))%type.
+  Definition JoystickMonitorSpec : Fiat.ADT.Core.ADT (RADLM_ADTSig JoystickMonitorNode unit) :=
+        ADTRep unit
            { Def Constructor RADL_Init (_ : unit) : rep := ret tt,
-             Def Method RADL_Step (r : rep, in_t : unit * Message (RADL_Subscriptions TriggerMonitorNode)) : _ :=
-               turret <- callMeth TriggerSpec RADL_Step (fst in_t) (snd in_t);
-             ret (tt, turret)
+             Def Method RADL_Step (r : rep, msg : unit * cRep (radlm_in_t JoystickMonitorNode) * cRep (radlm_monitor_in_t JoystickMonitorNode)) : JoystickMonitor_Output :=
+               joystick <- callMeth JoystickSpec RADL_Step (fst (fst msg)) (snd (fst msg));
+             ret (tt, (joystick, inil _ ))
            }.
 
   (* After Refinement, we arrive at an implementation which simply calls the monitor functions,
      with each function enforcing the global guard locally. *)
-  Definition PaintballImpl :
-  ADTRep (Rep BarrelMonitorSpec * Rep TriggerMonitorSpec *
-              Rep TurretMonitorSpec * Rep BarrelSpec *
-              Rep TriggerSpec * Rep TurretSpec)
-      { Def Constructor RADL_Init (_: ()) : rep :=
-          barrel <- (callCons BarrelSpec RADL_Init) ();
-          turret <- (callCons TurretSpec RADL_Init) ();
-          trigger <- (callCons TriggerSpec RADL_Init) ();
-          barrelmonitor <- (callCons BarrelMonitorSpec RADL_Init) ();
-          turretmonitor <- (callCons TurretMonitorSpec RADL_Init) ();
-          triggermonitor <- (callCons TriggerMonitorSpec RADL_Init) ();
-          ret
-            (barrelmonitor, turretmonitor, triggermonitor, barrel, turret,
-            trigger) ,
-        Def Method RADL_Step (r : rep, in_t : (Message PaintballTopicIDs)) :
-        (Message PaintballTopicIDs) :=
-          barrel <- (callMeth BarrelMonitorSpec RADL_Step)
-                      (snd r)
-                      ((),
-                      SubMessage
-                        [``(``("Trigger")); ``(``("TiltX")); ``(``("TiltY"))]
-                        in_t);
-          turret <- (callMeth TurretMonitorSpec RADL_Step)
-                      (snd r) ((), SubMessage [] in_t);
-          trigger <- (callMeth TriggerMonitorSpec RADL_Step)
-                       (snd r) ((), SubMessage [] in_t);
-          ret
-            (fst barrel, fst turret, fst trigger, fst (snd barrel),
-            fst (snd turret), fst (snd trigger),
-            ilist_app (snd (snd turret))
-              (ilist_app (snd (snd trigger)) (snd (snd barrel))))  })
 
   (* This implementation includes a list of monitor node specs from which we
      can derive Gallina implementations. Eventually (hopefully soon) we can
      then plug these into our pipeline to produce Bedrock implementations which
      can be integrated into the monitor framework. *)
 
-  Definition PaintballImpl :
-    MostlySharpened PaintballSpec.
+  Definition ExampleImpl :
+    MostlySharpened ExampleSpec.
   Proof.
     start sharpening ADT.
-    hone representation using (fun (r_o : Rep PaintballSpec)
+    hone representation using (fun (r_o : Rep ExampleSpec)
                                    (r_n :
-                                      Rep BarrelMonitorSpec *
-                                      Rep TriggerMonitorSpec *
+                                      Rep PaintballMonitorSpec *
+                                      Rep JoystickMonitorSpec *
                                       Rep TurretMonitorSpec *
-                                      Rep BarrelSpec *
-                                      Rep TriggerSpec *
+                                      Rep PaintballSpec *
+                                      Rep JoystickSpec *
                                       Rep TurretSpec)
                                         => True).
     { subst H.
-      instantiate (1 := fun d => barrel <- (callCons BarrelSpec RADL_Init) ();
+      instantiate (1 := fun d => barrel <- (callCons PaintballSpec RADL_Init) ();
                    turret <- (callCons TurretSpec RADL_Init) ();
-                   trigger <- (callCons TriggerSpec RADL_Init) ();
-                   barrelmonitor <- (callCons BarrelMonitorSpec RADL_Init) ();
+                   trigger <- (callCons JoystickSpec RADL_Init) ();
+                   barrelmonitor <- (callCons PaintballMonitorSpec RADL_Init) ();
                    turretmonitor <- (callCons TurretMonitorSpec RADL_Init) ();
-                   triggermonitor <- (callCons TriggerMonitorSpec RADL_Init) ();
+                   triggermonitor <- (callCons JoystickMonitorSpec RADL_Init) ();
                    ret (barrelmonitor, turretmonitor, triggermonitor, barrel, turret, trigger)).
       simplify with monad laws; refine pick val ( (), (), (), (), (), ()); eauto; simpl.
       intros v Comp_v; computes_to_inv; subst; eauto.
     }
-    {
-      subst H0; instantiate (1 := fun (r : Rep BarrelMonitorSpec *
-                                      Rep TriggerMonitorSpec *
-                                      Rep TurretMonitorSpec *
-                                      Rep BarrelSpec *
-                                      Rep TriggerSpec *
-                                      Rep TurretSpec)  (in_t : Message PaintballTopicIDs) =>
-              barrel <- callMeth BarrelMonitorSpec RADL_Step (snd r) (tt, (SubMessage [````"Trigger";
-                                                                                         ````"TiltX";
-                                                                                         ````"TiltY"] in_t));
-        turret <- callMeth TurretMonitorSpec RADL_Step (snd r) (tt, SubMessage [] in_t);
-        trigger <- callMeth TriggerMonitorSpec RADL_Step (snd r) (tt, SubMessage [] in_t);
-        ret ((fst barrel, fst turret, fst trigger, fst (snd barrel), fst (snd turret), fst (snd trigger)),
-             (ilist_app (snd (snd turret)) (ilist_app (snd (snd trigger)) (snd (snd barrel)))))).
-      simpl.
-      unfold eq_rect_r, eq_rect, eq_sym.
-      simpl.
+    { subst H0.
+      instantiate (1 :=  fun (r : Rep PaintballMonitorSpec *
+                                 Rep JoystickMonitorSpec *
+                                 Rep TurretMonitorSpec *
+                                 Rep PaintballSpec *
+                                 Rep JoystickSpec *
+                                 Rep TurretSpec)
+                            (msg : Message PaintballTopicIDs) =>
+       barrel <- callMeth PaintballMonitorSpec RADL_Step (snd r) (tt, SubMessage ["Trigger"] msg,
+                                                                  SubMessage ["TiltX";
+                                                                               "TiltY"] msg);
+        turret <- callMeth TurretMonitorSpec RADL_Step (snd r) (tt, SubMessage [] msg, SubMessage [] msg);
+        trigger <- callMeth JoystickMonitorSpec RADL_Step (snd r) (tt, SubMessage [] msg, SubMessage [] msg);
+        ret ((fst barrel, fst turret, fst trigger, fst (fst (snd barrel)), fst (fst (snd turret)), fst (fst (snd trigger))),
+             (ilist_app (snd (fst (snd turret))) (ilist_app (snd (fst (snd trigger))) (snd (fst (snd barrel))))))).
       admit.
     }
+    (* This is essentially what the final goal should look like.*)
+  Admitted.
 
-    simpl in H0.
-      simpl in c.
-      unfold methodType in H0.
-      simpl in H0.
-      unfold PaintballTopicIDs in H0.
-      simpl in H0.
-      eauto.
-    simpl; rewrite <- refineEquiv_bind_unit.
-    rewrite <- refineEquiv_bind_unit.
-    simplify with monad laws.
-    simpl in *.
-    unfold PaintballSpec.
-
-
-  econstructor.
-    repeat econstructor.
-
-
-    econstructor.
-    simpl in *.
-    simpl.
-
-
-
-End Paintball.
+End Example.
