src/Fiat4Monitors/MonitorADTs.v
@@ -1,0 +1,291 @@
+Set Implicit Arguments.
+
+Require Import Coq.Lists.List Coq.Program.Program Coq.Arith.Arith.
+Require Import Fiat.Fiat4Monitors.RADL_Definitions
+        Fiat.Fiat4Monitors.TurretMonitorSpec
+        Fiat.ADT
+        Fiat.ADT.ComputationalADT
+        Fiat.ADTNotation
+        Fiat.ADTRefinement
+        Fiat.ADTRefinement.BuildADTRefinements.
+Require Import Bedrock.Platform.Facade.DFacade.
+Require Import Bedrock.Platform.Facade.Notations.
+Require Import Bedrock.Platform.Cito.ADT.
+Require Import Bedrock.Platform.Cito.RepInv.
+
+Ltac crush_types :=
+  unfold type_conforming, same_types, same_type; intros;
+  repeat match goal with
+           | [ H: exists t, _ |- _ ] => destruct H
+         end; subst;
+  intuition.
+
+Section MonitorADTs.
+(* Each of these structs is represented in Facade as a distinct ADT. *)
+  Variable Topics : list RADL_Topic. (* List of Topics in the Network. *)
+  Variable MonitorNode : RADLM_Node Topics. (* The Monitor Node we're modelling. *)
+
+  (* The Specificaiton of Monitor Node we're modelling. *)
+  Variable MonitorNodeSpec :
+    Fiat.ADT.Core.ADT (RADLM_ADTSig MonitorNode unit).
+
+  Inductive MonitorADTValues : Type :=
+  | Message_In : cRep (radlm_in_t MonitorNode) -> MonitorADTValues
+  | Message_Out : cRep (radlm_out_t MonitorNode) -> MonitorADTValues
+  | Message_Monitor_In : cRep (radlm_monitor_in_t MonitorNode) -> MonitorADTValues
+  | Message_Monitor_Out : cRep (radlm_monitor_out_t MonitorNode) -> MonitorADTValues
+  | RADL_Monitored_Node : unit -> MonitorADTValues
+  | RADLM_Node : Rep MonitorNodeSpec -> MonitorADTValues.
+
+  (* Specs for getters and setters for each message type . *)
+  Section Message_In_Specs.
+    (* Coercions for getter domain and codomain values. *)
+    Let topics := RADL_Subscriptions (RADLM_MonitoredNode MonitorNode).
+    Variable idx : BoundedIndex
+                     (map (fun id : BoundedIndex topics => bindex id)
+                          (LiftTopics (Topics := Topics) topics)).
+    Variable Get_In_DomMap
+    : unit -> fst (MethodDomCod (MessageADTSig topics) (BuildGetMethodID topics idx)) .
+    Variable Get_In_CodMap
+    : snd (MethodDomCod (MessageADTSig topics) (BuildGetMethodID topics idx))
+      -> Memory.W.
+    Definition Message_In_GetSpec
+    : AxiomaticSpec MonitorADTValues.
+      refine {|
+          PreCond args := exists msg, args = [ADT (Message_In msg)];
+          PostCond args ret :=
+            exists msg, args = [(ADT (Message_In msg),
+                                 Some (Message_In msg)) ] /\
+                        ret = SCA _
+                                  (Get_In_CodMap (snd (CallMessageGetMethod msg idx (Get_In_DomMap tt))))
+        |}; crush_types.
+    Defined.
+
+    (* Coercions for setter domain and codomain values. *)
+    Variable Set_In_CodMap
+    : Memory.W -> fst
+                    (MethodDomCod
+                       (MessageADTSig topics)
+                       (BuildSetMethodID topics idx)).
+
+    Definition Message_In_SetSpec
+    : AxiomaticSpec MonitorADTValues.
+      refine {|
+          PreCond args := exists msg w, args = [ADT (Message_In msg), SCA _ w];
+          PostCond args ret :=
+            exists msg w, args = [(ADT (Message_In msg),
+                                   Some (Message_In (fst (CallMessageSetMethod msg idx (Set_In_CodMap w))))),
+                                  (SCA _ w, None)
+                                 ]
+        |}; crush_types.
+    Defined.
+  End Message_In_Specs.
+
+  Section Message_Out_Specs.
+    (* Coercions for getter domain and codomain values. *)
+    Let topics := RADL_Publications (RADLM_MonitoredNode MonitorNode).
+    Variable idx : BoundedIndex
+                      (map (fun id : BoundedIndex topics => bindex id)
+                           (LiftTopics (Topics := Topics) topics)).
+    Variable Get_Out_DomMap
+    : unit -> fst (MethodDomCod (MessageADTSig topics) (BuildGetMethodID topics idx)) .
+    Variable Get_Out_CodMap
+    : snd (MethodDomCod (MessageADTSig topics) (BuildGetMethodID topics idx))
+      -> Memory.W.
+
+    Definition Message_Out_GetSpec
+    : AxiomaticSpec MonitorADTValues.
+      refine {|
+          PreCond args := exists msg, args = [ADT (Message_Out msg)];
+          PostCond args ret :=
+            exists msg, args = [(ADT (Message_Out msg),
+                                 Some (Message_Out msg)) ] /\
+                        ret = SCA _
+                                  (Get_Out_CodMap
+                                                  (snd (CallMessageGetMethod msg idx (Get_Out_DomMap tt))))
+        |}; crush_types.
+    Defined.
+
+    (* Coercions for setter domain and codomain values. *)
+    Variable Set_Out_CodMap
+    : Memory.W -> fst
+                      (MethodDomCod
+                         (MessageADTSig topics)
+                         (BuildSetMethodID topics idx)).
+
+    Definition Message_Out_SetSpec
+    : AxiomaticSpec MonitorADTValues.
+      refine {|
+          PreCond args := exists msg w, args = [ADT (Message_Out msg), SCA _ w];
+          PostCond args ret :=
+            exists msg w, args = [(ADT (Message_Out msg),
+                                   Some (Message_Out (fst (CallMessageSetMethod msg idx (Set_Out_CodMap w))))),
+                                  (SCA _ w, None)
+                                 ]
+        |}; crush_types.
+    Defined.
+  End Message_Out_Specs.
+
+  Section Message_Monitor_In_Specs.
+    (* Coercions for getter domain and codomain values. *)
+    Let topics := RADLM_Subscriptions MonitorNode.
+    Variable idx : BoundedIndex
+                      (map (fun id : BoundedIndex topics => bindex id)
+                           (LiftTopics (Topics := Topics) topics)).
+    Variable Get_Monitor_In_DomMap
+    : unit -> fst (MethodDomCod (MessageADTSig topics) (BuildGetMethodID topics idx)) .
+    Variable Get_Monitor_In_CodMap
+    : snd (MethodDomCod (MessageADTSig topics) (BuildGetMethodID topics idx))
+      -> Memory.W.
+    Definition Message_Monitor_In_GetSpec
+    : AxiomaticSpec MonitorADTValues.
+      refine {|
+          PreCond args := exists msg, args = [ADT (Message_Monitor_In msg)];
+          PostCond args ret :=
+            exists msg, args = [(ADT (Message_Monitor_In msg),
+                                 Some (Message_Monitor_In msg)) ] /\
+                        ret = SCA _
+                                  (Get_Monitor_In_CodMap
+                                                 (snd (CallMessageGetMethod msg idx (Get_Monitor_In_DomMap tt))))
+        |}; crush_types.
+    Defined.
+
+    (* Coercions for setter domain and codomain values. *)
+    Variable Set_Monitor_In_CodMap
+    : Memory.W -> fst
+                      (MethodDomCod
+                         (MessageADTSig topics)
+                         (BuildSetMethodID topics idx)).
+
+    Definition Message_Monitor_In_SetSpec
+    : AxiomaticSpec MonitorADTValues.
+      refine {|
+          PreCond args := exists msg w, args = [ADT (Message_Monitor_In msg), SCA _ w];
+          PostCond args ret :=
+            exists msg w, args = [(ADT (Message_Monitor_In msg),
+                                   Some (Message_Monitor_In (fst (CallMessageSetMethod msg idx (Set_Monitor_In_CodMap w))))),
+                                  (SCA _ w, None)
+                                 ]
+        |}; crush_types.
+    Defined.
+  End Message_Monitor_In_Specs.
+
+  Section Message_Monitor_Out_Specs.
+    (* Coercions for getter domain and codomain values. *)
+    Let topics := RADLM_Publications MonitorNode.
+    Variable idx : BoundedIndex
+                      (map (fun id : BoundedIndex topics => bindex id)
+                           (LiftTopics (Topics := Topics) topics)).
+    Variable Get_Monitor_Out_DomMap
+    : unit -> fst (MethodDomCod (MessageADTSig topics) (BuildGetMethodID topics idx)) .
+    Variable Get_Monitor_Out_CodMap
+    : snd (MethodDomCod (MessageADTSig topics) (BuildGetMethodID topics idx))
+      -> Memory.W.
+    Definition Message_Monitor_Out_GetSpec
+    : AxiomaticSpec MonitorADTValues.
+      refine {|
+          PreCond args := exists msg, args = [ADT (Message_Monitor_Out msg)];
+          PostCond args ret :=
+            exists msg, args = [(ADT (Message_Monitor_Out msg),
+                                 Some (Message_Monitor_Out msg)) ] /\
+                        ret = SCA _
+                                  (Get_Monitor_Out_CodMap
+                                                 (snd (CallMessageGetMethod msg idx (Get_Monitor_Out_DomMap tt))))
+        |}; crush_types.
+    Defined.
+
+    (* Coercions for setter domain and codomain values. *)
+    Variable Set_Monitor_Out_CodMap
+    : Memory.W -> fst
+                      (MethodDomCod
+                         (MessageADTSig topics)
+                         (BuildSetMethodID topics idx)).
+
+    Definition Message_Monitor_Out_SetSpec
+    : AxiomaticSpec MonitorADTValues.
+      refine {|
+          PreCond args := exists msg w, args = [ADT (Message_Monitor_Out msg), SCA _ w];
+          PostCond args ret :=
+            exists msg w, args = [(ADT (Message_Monitor_Out msg),
+                                   Some (Message_Monitor_Out (fst (CallMessageSetMethod msg idx (Set_Monitor_Out_CodMap w))))),
+                                  (SCA _ w, None)
+                                 ]
+        |}; crush_types.
+    Defined.
+  End Message_Monitor_Out_Specs.
+
+  Definition RADL_Monitored_Node_StepSpec
+  : AxiomaticSpec MonitorADTValues.
+    refine {|
+        PreCond args :=
+          exists node in_msg out_msg,
+            args = [ADT (RADL_Monitored_Node node);
+                     ADT (Message_In in_msg);
+                     ADT (Message_Out out_msg) ];
+        PostCond args ret :=
+          exists node in_msg out_msg in_msg' out_msg',
+            args = [(ADT (RADL_Monitored_Node node),
+                     Some (RADL_Monitored_Node node));
+                     (ADT (Message_In in_msg),
+                      Some (Message_In in_msg'));
+                     (ADT (Message_Out out_msg),
+                      Some (Message_Out out_msg'))]
+      |}; crush_types.
+  Defined.
+
+  (* The Monitor Node's constructor and step method 
+     both satisfy the Fiat specifications. *)
+  Definition MonitorNode_InitSpec :
+    AxiomaticSpec MonitorADTValues.
+    refine {| PreCond args :=
+                args = [];
+              PostCond args ret :=
+                exists monitor_node,
+                  args = [ ]
+                  /\ ret = ADT (RADLM_Node monitor_node)
+                  /\ computes_to (callCons MonitorNodeSpec RADL_Init ())
+                                 monitor_node |}; crush_types.
+  Defined.
+
+  Definition MonitorNode_StepSpec :
+    AxiomaticSpec MonitorADTValues.
+    refine {| PreCond args :=
+                exists monitor_node node
+                       in_msg out_msg
+                       monitor_in_msg monitor_out_msg,
+                  args = [
+                    ADT (RADLM_Node monitor_node);
+                    ADT (RADL_Monitored_Node node);
+                    ADT (Message_In in_msg);
+                    ADT (Message_Out out_msg);
+                    ADT (Message_Monitor_In monitor_in_msg);
+                    ADT (Message_Monitor_Out monitor_out_msg)
+                  ];
+              PostCond args ret :=
+                exists monitor_node node
+                       in_msg out_msg
+                       monitor_in_msg monitor_out_msg
+                       monitor_node'  node' out_msg' monitor_out_msg',
+                  args = [(ADT (RADLM_Node monitor_node),
+                           Some (RADLM_Node monitor_node'));
+                           (ADT (RADL_Monitored_Node node),
+                            Some (RADL_Monitored_Node node'));
+                           (ADT (Message_In in_msg),
+                            Some (Message_In in_msg));
+                           (ADT (Message_Out out_msg),
+                            Some (Message_Out out_msg'));
+                           (ADT (Message_Monitor_In monitor_in_msg),
+                            Some (Message_Monitor_In monitor_in_msg));
+                           (ADT (Message_Monitor_Out monitor_out_msg),
+                            Some (Message_Monitor_Out monitor_out_msg'))
+                         ]
+                  /\ computes_to (callMeth MonitorNodeSpec RADL_Step monitor_node (node, in_msg, monitor_in_msg))
+                                 (monitor_node', (node', out_msg', monitor_out_msg'))
+           |}; crush_types.
+  Defined.
+
+End MonitorADTs.
+
+Module Adt <: ADT.
+  Definition ADTValue := MonitorADTValues (PaintballMonitorSpec (fun _ => true) (fun _ => true)).
+End Adt.
