src/Fiat4Monitors/MonitorRepInv.v
@@ -1,0 +1,39 @@
+Set Implicit Arguments.
+
+Require Import Coq.Lists.List Coq.Program.Program Coq.Arith.Arith.
+Require Import Fiat.Fiat4Monitors.RADL_Definitions
+        Fiat.Fiat4Monitors.TurretMonitorSpec
+        Fiat.Fiat4Monitors.MonitorADTs
+        Fiat.ADT
+        Fiat.ADT.ComputationalADT
+        Fiat.ADTNotation
+        Fiat.ADTRefinement
+        Fiat.ADTRefinement.BuildADTRefinements.
+Require Import Bedrock.Platform.Facade.DFacade.
+Require Import Bedrock.Platform.Facade.Notations.
+Require Import Bedrock.Platform.Cito.ADT.
+Require Import Bedrock.Platform.Cito.RepInv.
+Require Import Bedrock.Platform.AutoSep.
+Set Implicit Arguments.
+
+Import Adt.
+
+(* This is a placeholder for a legitimate description of the memory layout. *)
+Definition Monitors_rep_inv p (adtvalue : ADTValue) : HProp :=
+  match adtvalue with
+    | _ => p =?> 1
+  end%Sep.
+
+Module Ri <: RepInv Adt.
+
+  Definition RepInv := W -> ADTValue -> HProp.
+
+  Definition rep_inv := Monitors_rep_inv.
+
+  Lemma rep_inv_ptr : forall p a, rep_inv p a ===> p =?> 1 * any.
+    destruct a;
+    unfold rep_inv, Monitors_rep_inv; simpl;
+    sepLemma; apply any_easy.
+  Qed.
+
+End Ri.
